refactor SimRelAddJF

Coq/src/SimRelAddJF.v
@@ -9,7 +9,7 @@ From imm Require Import Events Execution
      imm_common imm_s imm_s_hb SimulationRel
      CertExecution2 CertExecutionMain
      SubExecution CombRelations AuxRel.
-Require Import AuxRel AuxDef EventStructure BasicStep Step Consistency 
+Require Import AuxRel AuxDef EventStructure BasicStep Step Consistency Execution
         LblStep CertRf CertGraph EventToAction ImmProperties
         SimRelCont SimRelEventToAction 
         SimRel SimRelCert SimRelCertBasicStep. 
@@ -23,8 +23,7 @@ Section SimRelAddJF.
   Variable sc : relation actid.
   Variable TC : trav_config.
   Variable TC' : trav_config.
-  Variable f : actid -> eventid.
-  Variable h : actid -> eventid.
+  Variable X : eventid -> Prop.
 
   Notation "'SE' S" := S.(ES.acts_set) (at level 10).
   Notation "'SEinit' S" := S.(ES.acts_init_set) (at level 10).
@@ -114,20 +113,25 @@ Section SimRelAddJF.
   Notation "'thread_cont_st' tid" :=
     (fun st => existT _ (thread_lts tid) st) (at level 10, only parsing).
 
-  Definition sim_add_jf thread st (w r' : eventid) (S S' : ES.t) : Prop :=
+  Notation "'kE' S" := (fun k => ES.cont_sb_dom S k) (at level 1, only parsing).
+  Notation "'ktid' S" := (fun k => ES.cont_thread S k) (at level 1, only parsing).
+
+  Notation "'certX' S" := (fun k => (X ∩₁ SNTid_ S (ktid S k)) ∪₁ (kE S k)) (at level 1, only parsing).
+
+  Definition sim_add_jf k (w r' : eventid) (S S' : ES.t) : Prop :=
     ⟪ rE' : SE S' r' ⟫ /\
     ⟪ rR' : SR S' r' ⟫ /\
-    ⟪ hCertDOM : (h □₁ (cert_dom G TC thread st)) w ⟫ /\
-    ⟪ CertRF : (cert_rf G sc TC' thread) (e2a S' w) (e2a S' r') ⟫ /\
+    ⟪ CertEx : certX S k w ⟫ /\
+    ⟪ CertRF : (cert_rf G sc TC' (ktid S k)) (e2a S' w) (e2a S' r') ⟫ /\
     ⟪ JF' : Sjf S' ≡ Sjf S ∪ ESstep.jf_delta w r' ⟫.
 
   Section SimRelAddJFProps. 
 
     Lemma sim_add_jf_jf_ncf w k k' e e' S S' 
           (st st' st'' : thread_st (ES.cont_thread S k))
-          (SRCC : simrel_cert prog S G sc TC TC' f h k st st'') 
+          (SRCC : simrel_cert prog S G sc TC TC' X k st st'') 
           (BSTEP_ : ESBasicStep.t_ (thread_lts (ES.cont_thread S k)) k k' st st' e e' S S') 
-          (SAJF : sim_add_jf (ES.cont_thread S k) st w e S S')
+          (SAJF : sim_add_jf k w e S S')
           (CST_REACHABLE : (lbl_step (ES.cont_thread S k))＊ st' st'') :
       Sjf S' ∩ Scf S' ≡ ∅₂.
     Proof. 
@@ -154,15 +158,59 @@ Section SimRelAddJF.
       2-4 : by ESBasicStep.step_solver.
 
       unfolder. ins. desf.
-      eapply cfk_hdom; eauto.  
+      eapply certX_ncf_cont; eauto.
       basic_solver.
     Qed.
+    
+    Lemma sim_add_jf_iss_sb_w w k k' e e' S S' 
+          (st st' st'' : thread_st (ES.cont_thread S k))
+          (SRCC : simrel_cert prog S G sc TC TC' X k st st'') 
+          (BSTEP_ : ESBasicStep.t_ (thread_lts (ES.cont_thread S k)) k k' st st' e e' S S') 
+          (SAJF : sim_add_jf k w e S S')
+          (CST_REACHABLE : (lbl_step (ES.cont_thread S k))＊ st' st'') :
+      ((X ∩₁ SNTid_ S (ktid S k) ∩₁ e2a S ⋄₁ I) ∪₁ ES.cont_sb_dom S k) w. 
+    Proof. 
+      assert (ESBasicStep.t e e' S S') as BSTEP.
+      { econstructor. eauto. }
+      assert (ES.Wf S) as WF.
+      { apply SRCC. }
+      cdes BSTEP_; cdes SAJF. 
+      assert (SE S w) as SEw.
+      { eapply cert_ex_inE; eauto. }
+      assert (e2a S' w = e2a S w) as e2aEQw.
+      { eapply basic_step_e2a_eq_dom; eauto. }
+      rewrite e2aEQw in *.
+      eapply cert_rf_ntid_iss_sb in CertRF.
+      2-6 : apply SRCC.
+      destruct CertRF as [Iss | SB].
+      { unfolder. left. 
+        unfolder in Iss. 
+        unfolder in CertEx. 
+        destruct Iss as [[NTID Iss] _].
+        destruct CertEx as [[Xw NTIDw] | KSBw]; auto.
+        eapply ES.cont_sb_tid in KSBw; eauto.
+        destruct KSBw as [INITw | TIDw].
+        { splits; auto.
+          { eapply Execution.init_in_ex; eauto. apply SRCC. }
+          destruct INITw as [_ TIDw]. rewrite TIDw.
+          intros kTID. eapply ktid_ninit; eauto. }
+        exfalso. apply NTID.
+        by rewrite <- e2a_tid. }
+      right. 
+      destruct CertEx as [[Xw NTIDw] | KSBw]; auto.
+      edestruct sb_tid_init as [STID | INITx]; eauto. 
+      { exfalso. apply NTIDw.
+        rewrite e2a_tid, STID, <- e2a_tid. 
+        erewrite ESBasicStep.basic_step_tid_e; eauto. }
+      eapply ES.cont_sb_dom_Einit; eauto.
+      admit. 
+    Admitted.
 
     Lemma weaken_sim_add_jf w k k' e e' S S' 
           (st st' st'' : thread_st (ES.cont_thread S k))
-          (SRCC : simrel_cert prog S G sc TC TC' f h k st st'') 
+          (SRCC : simrel_cert prog S G sc TC TC' X k st st'') 
           (BSTEP_ : ESBasicStep.t_ (thread_lts (ES.cont_thread S k)) k k' st st' e e' S S') 
-          (SAJF : sim_add_jf (ES.cont_thread S k) st w e S S') 
+          (SAJF : sim_add_jf k w e S S') 
           (CST_REACHABLE : (lbl_step (ES.cont_thread S k))＊ st' st'') : 
       ESstep.add_jf w e S S'.
     Proof. 
@@ -173,7 +221,7 @@ Section SimRelAddJF.
       assert (ES.Wf S) as WF.
       { apply SRCC. }
       assert (SE S w) as SEw.
-      { eapply a2e_img; eauto. apply SRCC. }
+      { eapply cert_ex_inE; eauto. }
       assert (SE S' w) as SEw'.
       { eapply ESBasicStep.basic_step_acts_set; eauto. basic_solver. }
       assert (SE S' e) as SEe'.
@@ -201,186 +249,67 @@ Section SimRelAddJF.
       { assert (same_val (certLab G st'') (e2a S' w) (e2a S' e)) as SAME_VAL.
         { eapply cert_rfv_clab; eauto. apply SRCC. }
         unfold same_val, val in *.
-        erewrite basic_step_e2a_certlab_e with (e := e); eauto.
+        erewrite basic_step_e2a_certlab_e 
+          with (e := e); eauto; try apply SRCC.
         arewrite (Slab S' w = Slab S w).
         { erewrite ESBasicStep.basic_step_lab_eq_dom; eauto. }
         assert (e2a S w = e2a S' w) as E2Aw. 
         { symmetry. eapply basic_step_e2a_eq_dom; eauto. }
         rewrite <- E2Aw in *.
-        eapply cert_rf_ntid_iss_sb in CertRF. 
-        2-10: apply SRCC.
-        unfolder in hCertDOM. destruct hCertDOM as [wa [CERTwa Hwa]].
-        assert (e2a S w = wa) as Gwwa.
-        { rewrite <- Hwa.
-          eapply a2e_fix; [apply SRCC|].
-          unfolder. basic_solver. }
-        arewrite (Slab S w = certLab G st'' (e2a S w)); [|auto].
-        rewrite <- Hwa at 1.
-        rewrite Gwwa.
-        arewrite ((Slab S) (h wa) = (Slab S ∘ h) wa).
-        destruct CertRF as [Iss | SB].
-        { assert (I wa) as Iw.
-          { apply seq_eqv_l in Iss. unfolder in Iss. rewrite <- Gwwa. basic_solver. }
-          unfold certLab.
-          destruct 
-            (excluded_middle_informative (acts_set (ProgToExecution.G st'') wa)) 
-            as [GCE | nGCE].
-          { assert (GNtid_ (ES.cont_thread S k) wa) as HH.
-            { apply seq_eqv_l in Iss. 
-              destruct Iss as [[NTID _] _].
-              rewrite <- Gwwa. apply NTID. }
-            exfalso. apply HH. 
-            eapply dcertE in GCE; [|apply SRCC].
-              by destruct GCE. }
-          eapply hlabCI; eauto.
-          basic_solver. }
-        edestruct sb_tid_init as [STID | INITx]; eauto. 
-        { eapply hlab; eauto. right. 
-          destruct CERTwa as [[Cwa | Iwa] | ACTSst]; auto.
-          { eapply cstate_covered; [apply SRCC|].
-            split; auto.
-              by rewrite <- Gwwa, STID, GTIDe. }
-          exfalso. destruct Iwa as [_ NTIDwa].
-          apply NTIDwa.
-          rewrite <- Gwwa.
-          erewrite <- ESBasicStep.basic_step_tid_e; eauto.
-            by rewrite e2a_tid. }
-        assert (C wa) as Cwa.
-        { eapply init_covered; [apply SRCC|].
-          rewrite <- Gwwa. 
-          split; auto.  
-          eapply e2a_GE; [apply SRCC|].
-          unfolder. eauto. }
-        eapply hlab; eauto. basic_solver. }
+        edestruct sim_add_jf_iss_sb_w
+          as [[[Xw NTIDw] Iw] | kSBw]; eauto. 
+        { erewrite cert_ex_cov_iss_cert_lab; 
+            [| apply SRCC |].
+          { unfold compose. by rewrite SAME_VAL. }
+          split; auto.
+          unfolder. right.
+          admit. }
+        erewrite kE_cert_lab; [| apply SRCC | auto].
+        unfold compose. by rewrite SAME_VAL. }
       intros CF.
       eapply sim_add_jf_jf_ncf; eauto.
       split; eauto.
       apply JF'. 
       autounfold with ESStepDb.
       basic_solver.
-    Qed.
-
-    Lemma sim_add_jf_iss_sb w k k' e e' S S' 
-          (st st' st'' : thread_st (ES.cont_thread S k))
-          (SRCC : simrel_cert prog S G sc TC TC' f h k st st'') 
-          (BSTEP_ : ESBasicStep.t_ (thread_lts (ES.cont_thread S k)) k k' st st' e e' S S') 
-          (SAJF : sim_add_jf (ES.cont_thread S k) st w e S S')
-          (CST_REACHABLE : (lbl_step (ES.cont_thread S k))＊ st' st'') :
-      (h □₁ (I ∩₁ (GNtid_ (ES.cont_thread S k))) ∪₁ ES.cont_sb_dom S k) w. 
-    Proof. 
-      assert (ESstep.add_jf w e S S') as AJF. 
-      { eapply weaken_sim_add_jf; eauto. } 
-      assert (ESBasicStep.t e e' S S') as BSTEP.
-      { econstructor. eauto. }
-      assert (ES.Wf S) as WF.
-      { apply SRCC. }
-      cdes BSTEP_; cdes SAJF; cdes AJF. 
-      assert (e2a S' w = e2a S w) as e2aEQw.
-      { eapply basic_step_e2a_eq_dom; eauto. }
-      assert (h (e2a S w) = w) as he2aEQw.
-      { fold (compose h (e2a S) w).
-        eapply fixset_swap; eauto. 
-        apply SRCC. }
-      rewrite e2aEQw in *.
-      eapply cert_rf_ntid_iss_sb in CertRF.
-      2-6 : apply SRCC.
-      destruct CertRF as [Iss | SB].
-      { unfolder. left. 
-        unfolder in Iss. 
-        destruct Iss as [[NTID Iss] _].
-        eexists; splits; eauto. }
-      unfolder. right. 
-      edestruct sb_tid_init as [STID | INITw]; eauto. 
-      { assert ((SE S ∩₁ Stid_ S (ES.cont_thread S k)) w) as HH. 
-        { split; auto.
-          rewrite <- !e2a_tid in STID.
-          rewrite STID.
-          erewrite ESBasicStep.basic_step_tid_e; eauto. }
-        eapply ES.cont_thread_sb_cf in HH; eauto. 
-        destruct HH as [HA | HB].
-        { generalize HA. basic_solver. }
-        exfalso. eapply cfk_hdom; eauto.
-        basic_solver. }
-      eapply ES.cont_sb_dom_Einit; eauto.
-      eapply himgInit; eauto.
-      unfolder; eexists; splits; eauto.
-      eapply wf_sbE, seq_eqv_lr in SB. 
-      basic_solver.
-    Qed.
+    Admitted.
 
     Lemma sim_add_jf_jf_delta_dom w k k' e e' S S' 
           (st st' st'' : thread_st (ES.cont_thread S k))
-          (SRCC : simrel_cert prog S G sc TC TC' f h k st st'') 
+          (SRCC : simrel_cert prog S G sc TC TC' X k st st'') 
           (BSTEP_ : ESBasicStep.t_ (thread_lts (ES.cont_thread S k)) k k' st st' e e' S S') 
-          (SAJF : sim_add_jf (ES.cont_thread S k) st w e S S')
+          (SAJF : sim_add_jf k w e S S')
           (CST_REACHABLE : (lbl_step (ES.cont_thread S k))＊ st' st'') :
-      dom_rel (ESstep.jf_delta w e) ⊆₁ h □₁ (cert_dom G TC (ES.cont_thread S k) st).
+      dom_rel (ESstep.jf_delta w e) ⊆₁ certX S k.
     Proof. 
       autounfold with ESStepDb.
-      edestruct sim_add_jf_iss_sb as [Iss | SB]; eauto. 
-      { unfold cert_dom. generalize Iss. basic_solver 10. }
-      eapply cont_sb_dom_in_hhdom in SB; eauto.
-      basic_solver.
+      rewrite dom_singl_rel.
+      intros w' EQw'. subst w'.
+      edestruct sim_add_jf_iss_sb_w as [Iss | SB]; eauto. 
+      { generalize Iss. basic_solver 10. }
+      by right.
     Qed.
 
     Lemma sim_add_jf_jfe_delta_dom w k k' e e' S S' 
           (st st' st'' : thread_st (ES.cont_thread S k))
-          (SRCC : simrel_cert prog S G sc TC TC' f h k st st'') 
+          (SRCC : simrel_cert prog S G sc TC TC' X k st st'') 
           (BSTEP_ : ESBasicStep.t_ (thread_lts (ES.cont_thread S k)) k k' st st' e e' S S') 
-          (SAJF : sim_add_jf (ES.cont_thread S k) st w e S S')
+          (SAJF : sim_add_jf k w e S S')
           (CST_REACHABLE : (lbl_step (ES.cont_thread S k))＊ st' st'') :
-      dom_rel (ESstep.jfe_delta S k w e) ⊆₁ h □₁ (I ∩₁ (GNtid_ (ES.cont_thread S k))).
+      dom_rel (ESstep.jfe_delta S k w e) ⊆₁ X ∩₁ SNTid_ S (ktid S k) ∩₁ e2a S ⋄₁ I. 
     Proof. 
       autounfold with ESStepDb.
-      edestruct sim_add_jf_iss_sb as [Iss | SB]; eauto. 
+      edestruct sim_add_jf_iss_sb_w as [Iss | SB]; eauto. 
       { generalize Iss. basic_solver 10. }
       unfolder. ins. desc. subst.
       exfalso. auto. 
     Qed.
 
-    (* Lemma sim_add_jf_jf_delta_ew w k k' e e' S S'  *)
-    (*       (st st' st'' : thread_st (ES.cont_thread S k)) *)
-    (*       (SRCC : simrel_cert prog S G sc TC TC' f h k st st'')  *)
-    (*       (BSTEP_ : ESBasicStep.t_ (thread_lts (ES.cont_thread S k)) k k' st st' e e' S S')  *)
-    (*       (SAJF : sim_add_jf (ES.cont_thread S k) st w e S S') *)
-    (*       (CST_REACHABLE : (lbl_step (ES.cont_thread S k))＊ st' st'') : *)
-    (*   ESstep.jf_delta w e ⊆ Sew S ⨾ ESstep.jf_delta w e. *)
-    (* Proof.  *)
-    (*   assert (ES.Wf S) as WF. *)
-    (*   { apply SRCC. } *)
-    (*   eapply weaken_sim_add_jf in SAJF; eauto. *)
-    (*   cdes SAJF. *)
-    (*   autounfold with ESStepDb. *)
-    (*   unfolder. ins. desf. *)
-    (*   eexists; splits; eauto. *)
-    (*   eapply ES.ew_refl; auto. *)
-    (*   basic_solver. *)
-    (* Qed. *)
-
-    (* Lemma sim_add_jf_jfe_delta_ew w k k' e e' S S'  *)
-    (*       (st st' st'' : thread_st (ES.cont_thread S k)) *)
-    (*       (SRCC : simrel_cert prog S G sc TC TC' f h k st st'')  *)
-    (*       (BSTEP_ : ESBasicStep.t_ (thread_lts (ES.cont_thread S k)) k k' st st' e e' S S')  *)
-    (*       (SAJF : sim_add_jf (ES.cont_thread S k) st w e S S') *)
-    (*       (CST_REACHABLE : (lbl_step (ES.cont_thread S k))＊ st' st'') : *)
-    (*   ESstep.jfe_delta S k w e ⊆ Sew S ⨾ ESstep.jfe_delta S k w e. *)
-    (* Proof.  *)
-    (*   assert (ES.Wf S) as WF. *)
-    (*   { apply SRCC. } *)
-    (*   eapply weaken_sim_add_jf in SAJF; eauto. *)
-    (*   cdes SAJF. *)
-    (*   autounfold with ESStepDb. *)
-    (*   unfolder. ins. desf. *)
-    (*   eexists; splits; eauto. *)
-    (*   eapply ES.ew_refl; auto. *)
-    (*   basic_solver. *)
-    (* Qed. *)
-
     Lemma sim_add_jf_e2a_jf_vf w k k' e e' S S' 
           (st st' st'' : thread_st (ES.cont_thread S k))
-          (SRCC : simrel_cert prog S G sc TC TC' f h k st st'') 
+          (SRCC : simrel_cert prog S G sc TC TC' X k st st'') 
           (BSTEP_ : ESBasicStep.t_ (thread_lts (ES.cont_thread S k)) k k' st st' e e' S S') 
-          (SAJF : sim_add_jf (ES.cont_thread S k) st w e S S')
+          (SAJF : sim_add_jf k w e S S')
           (CST_REACHABLE : (lbl_step (ES.cont_thread S k))＊ st' st'') :
       e2a S' □ Sjf S' ⊆ Gvf.
     Proof. 
@@ -403,12 +332,11 @@ Section SimRelAddJF.
 
     Lemma sim_add_jf_hb_sw_delta_dom w k k' e e' S S'
         (st st' st'': (thread_st (ES.cont_thread S k)))
-        (SRCC : simrel_cert prog S G sc TC TC' f h k st st'') 
+        (SRCC : simrel_cert prog S G sc TC TC' X k st st'') 
         (BSTEP_ : ESBasicStep.t_ (thread_lts (ES.cont_thread S k)) k k' st st' e e' S S') 
-        (SAJF : sim_add_jf (ES.cont_thread S k) st w e S S')
+        (SAJF : sim_add_jf k w e S S')
         (CST_REACHABLE : (lbl_step (ES.cont_thread S k))＊ st' st'') : 
-      dom_rel ((Shb S)^? ⨾ ESstep.sw_delta S S' k e e') ⊆₁ 
-              h □₁ cert_dom G TC (ES.cont_thread S k) st.
+      dom_rel ((Shb S)^? ⨾ ESstep.sw_delta S S' k e e') ⊆₁ certX S k.
     Proof. 
       cdes BSTEP_; cdes SAJF.
       assert (ESBasicStep.t e e' S S') as BSTEP.
@@ -429,19 +357,18 @@ Section SimRelAddJF.
         cdes SAJF. unfold ESstep.jf_delta. 
         unfolder. ins. desf. }
       etransitivity.
-      2 : eapply hb_rel_ew_hD; eauto.
+      2 : eapply hb_rel_ew_cert_ex; eauto.
       unfold ESstep.jf_delta. 
       basic_solver 20.
     Qed.
 
     Lemma sim_add_jf_hb_delta_dom w k k' e e' S S'
         (st st' st'': (thread_st (ES.cont_thread S k)))
-        (SRCC : simrel_cert prog S G sc TC TC' f h k st st'') 
+        (SRCC : simrel_cert prog S G sc TC TC' X k st st'') 
         (BSTEP_ : ESBasicStep.t_ (thread_lts (ES.cont_thread S k)) k k' st st' e e' S S') 
-        (SAJF : sim_add_jf (ES.cont_thread S k) st w e S S')
+        (SAJF : sim_add_jf k w e S S')
         (CST_REACHABLE : (lbl_step (ES.cont_thread S k))＊ st' st'') : 
-      dom_rel (ESstep.hb_delta S S' k e e') ⊆₁ 
-              h □₁ cert_dom G TC (ES.cont_thread S k) st ∪₁ eq e. 
+      dom_rel (ESstep.hb_delta S S' k e e') ⊆₁ certX S k ∪₁ eq e. 
     Proof. 
       cdes BSTEP_; cdes SAJF.
       assert (ESBasicStep.t e e' S S') as BSTEP.
@@ -456,48 +383,11 @@ Section SimRelAddJF.
       left; eapply sim_add_jf_hb_sw_delta_dom; eauto.
     Qed.
 
-    (* Lemma sim_add_jf_jf_ncf w k k' e e' S S'  *)
-    (*       (st st' st'' : thread_st (ES.cont_thread S k)) *)
-    (*       (SRCC : simrel_cert prog S G sc TC TC' f h k st st'')  *)
-    (*       (BSTEP_ : ESBasicStep.t_ (thread_lts (ES.cont_thread S k)) k k' st st' e e' S S')  *)
-    (*       (SAJF : sim_add_jf (ES.cont_thread S k) st w e S S') *)
-    (*       (CST_REACHABLE : (lbl_step (ES.cont_thread S k))＊ st' st'') : *)
-    (*   Sjf S' ∩ Scf S' ≡ ∅₂. *)
-    (* Proof.  *)
-    (*   assert (ESstep.add_jf w e S S') as AJF.  *)
-    (*   { eapply weaken_sim_add_jf; eauto. }  *)
-    (*   assert (ESBasicStep.t e e' S S') as BSTEP. *)
-    (*   { econstructor. eauto. } *)
-    (*   assert (ES.Wf S) as WF. *)
-    (*   { apply SRCC. } *)
-    (*   cdes BSTEP_; cdes SAJF; cdes AJF.  *)
-    (*   split; [|done]. *)
-    (*   rewrite JF'. *)
-    (*   erewrite ESBasicStep.basic_step_cf; eauto. *)
-    (*   rewrite !inter_union_l, !inter_union_r.  *)
-    (*   unionL. *)
-
-    (*   { apply ES.jf_ncf; apply SRCC. }  *)
-
-    (*   1-2 : by ESBasicStep.step_solver. *)
-
-    (*   autounfold with ESStepDb. *)
-    (*   rewrite !csE, !transp_cross. *)
-    (*   rewrite !inter_union_r.  *)
-    (*   unionL. *)
-
-    (*   2-4 : by ESBasicStep.step_solver. *)
-
-    (*   unfolder. ins. desf. *)
-    (*   eapply cfk_hdom; eauto.   *)
-    (*   basic_solver. *)
-    (* Qed. *)
-
     Lemma sim_add_jf_hb_jf_ncf w k k' e e' S S' 
           (st st' st'' : thread_st (ES.cont_thread S k))
-          (SRCC : simrel_cert prog S G sc TC TC' f h k st st'') 
+          (SRCC : simrel_cert prog S G sc TC TC' X k st st'') 
           (BSTEP_ : ESBasicStep.t_ (thread_lts (ES.cont_thread S k)) k k' st st' e e' S S') 
-          (SAJF : sim_add_jf (ES.cont_thread S k) st w e S S')
+          (SAJF : sim_add_jf k w e S S')
           (CST_REACHABLE : (lbl_step (ES.cont_thread S k))＊ st' st'') 
           (nF' : eq_opt e' ∩₁ SF S' ⊆₁ ∅) :
       (Shb S' ⨾ Sjf S') ∩ Scf S' ≡ ∅₂.
@@ -525,9 +415,9 @@ Section SimRelAddJF.
       unionL.
 
       { unfolder. ins. desf. 
-        eapply cfk_hdom; eauto. 
+        eapply certX_ncf_cont; eauto. 
         split; [|eauto]. 
-        eapply hb_hD; eauto. 
+        eapply cert_ex_hb_prcl; eauto. 
         basic_solver 10. }
 
       all : by ESBasicStep.step_solver. 
@@ -535,9 +425,9 @@ Section SimRelAddJF.
 
     Lemma sim_add_jf_hb_tjf_ncf w k k' e e' S S' 
           (st st' st'' : thread_st (ES.cont_thread S k))
-          (SRCC : simrel_cert prog S G sc TC TC' f h k st st'') 
+          (SRCC : simrel_cert prog S G sc TC TC' X k st st'') 
           (BSTEP_ : ESBasicStep.t_ (thread_lts (ES.cont_thread S k)) k k' st st' e e' S S') 
-          (SAJF : sim_add_jf (ES.cont_thread S k) st w e S S')
+          (SAJF : sim_add_jf k w e S S')
           (CST_REACHABLE : (lbl_step (ES.cont_thread S k))＊ st' st'') 
           (nF' : eq_opt e' ∩₁ SF S' ⊆₁ ∅) :
       (Shb S' ⨾ (Sjf S')⁻¹) ∩ Scf S' ≡ ∅₂.
@@ -573,8 +463,7 @@ Section SimRelAddJF.
       rewrite transp_singl_rel.
       intros x y [HH CF].
       destruct HH as [a [[b [certD HBd]] JFd]].
-      eapply a2e_ncf.
-      { apply SRCC.(sr_a2e_h). }
+      eapply cert_ex_ncf; eauto.
       apply seq_eqv_lr. 
       splits; [apply certD| apply CF |]. 
       unfold singl_rel in JFd. desf.
@@ -582,9 +471,9 @@ Section SimRelAddJF.
 
     Lemma sim_add_jf_hb_jf_thb_ncf w k k' e e' S S' 
           (st st' st'' : thread_st (ES.cont_thread S k))
-          (SRCC : simrel_cert prog S G sc TC TC' f h k st st'') 
+          (SRCC : simrel_cert prog S G sc TC TC' X k st st'') 
           (BSTEP_ : ESBasicStep.t_ (thread_lts (ES.cont_thread S k)) k k' st st' e e' S S') 
-          (SAJF : sim_add_jf (ES.cont_thread S k) st w e S S')
+          (SAJF : sim_add_jf k w e S S')
           (CST_REACHABLE : (lbl_step (ES.cont_thread S k))＊ st' st'') 
           (nF' : eq_opt e' ∩₁ SF S' ⊆₁ ∅) :
       (Shb S' ⨾ Sjf S' ⨾ (Shb S')⁻¹) ∩ Scf S' ≡ ∅₂.
@@ -622,11 +511,10 @@ Section SimRelAddJF.
       unfold ESstep.jf_delta.
       intros x y [HH CF].
       destruct HH as [a [HB [b [JFd HBd]]]].
-      eapply a2e_ncf.
-      { apply SRCC.(sr_a2e_h). }
+      eapply cert_ex_ncf; eauto.
       apply seq_eqv_lr. 
       splits; [|apply CF|].
-      { eapply hb_hD; eauto.
+      { eapply cert_ex_hb_prcl; eauto.
         unfolder in JFd. desc. subst a b.
         basic_solver 10. }
       unfold transp in HBd.
@@ -639,9 +527,9 @@ Section SimRelAddJF.
 
     Lemma sim_add_jf_jf_necf w k k' e e' S S' 
           (st st' st'' : thread_st (ES.cont_thread S k))
-          (SRCC : simrel_cert prog S G sc TC TC' f h k st st'') 
+          (SRCC : simrel_cert prog S G sc TC TC' X k st st'') 
           (BSTEP_ : ESBasicStep.t_ (thread_lts (ES.cont_thread S k)) k k' st st' e e' S S') 
-          (SAJF : sim_add_jf (ES.cont_thread S k) st w e S S')
+          (SAJF : sim_add_jf k w e S S')
           (CST_REACHABLE : (lbl_step (ES.cont_thread S k))＊ st' st'') 
           (nF' : eq_opt e' ∩₁ SF S' ⊆₁ ∅) :
       Sjf S' ∩ Secf S' ≡ ∅₂. 
@@ -655,9 +543,9 @@ Section SimRelAddJF.
     
     Lemma sim_add_jf_jfe_vis w k k' e e' S S' 
           (st st' st'' : thread_st (ES.cont_thread S k))
-          (SRCC : simrel_cert prog S G sc TC TC' f h k st st'') 
+          (SRCC : simrel_cert prog S G sc TC TC' X k st st'') 
           (BSTEP_ : ESBasicStep.t_ (thread_lts (ES.cont_thread S k)) k k' st st' e e' S S') 
-          (SAJF : sim_add_jf (ES.cont_thread S k) st w e S S') 
+          (SAJF : sim_add_jf k w e S S') 
           (CST_REACHABLE : (lbl_step (ES.cont_thread S k))＊ st' st'') : 
       dom_rel (Sjfe S') ⊆₁ vis S. 
     Proof. 
@@ -673,17 +561,18 @@ Section SimRelAddJF.
       apply set_subset_union_l. split. 
       { apply SRCC. }
       rewrite sim_add_jf_jfe_delta_dom; eauto.
-      etransitivity; [|eapply hvis]; eauto.
-      basic_solver 10.
+      erewrite Execution.ex_vis with (S := S) (X := X).
+      { basic_solver. }
+      apply SRCC.
     Qed.
 
     Lemma sim_add_jf_jfe_fI w k k' e e' S S' 
           (st st' st'' : thread_st (ES.cont_thread S k))
-          (SRCC : simrel_cert prog S G sc TC TC' f h k st st'') 
+          (SRCC : simrel_cert prog S G sc TC TC' X k st st'') 
           (BSTEP_ : ESBasicStep.t_ (thread_lts (ES.cont_thread S k)) k k' st st' e e' S S') 
-          (SAJF : sim_add_jf (ES.cont_thread S k) st w e S S') 
+          (SAJF : sim_add_jf k w e S S') 
           (CST_REACHABLE : (lbl_step (ES.cont_thread S k))＊ st' st'') : 
-      dom_rel (Sjfe S') ⊆₁ dom_rel (Sew S ⨾ ⦗ f □₁ I ⦘). 
+      dom_rel (Sjfe S') ⊆₁ dom_rel (Sew S ⨾ ⦗ X ∩₁ e2a S ⋄₁ I ⦘). 
     Proof. 
       assert (ES.Wf S) as WF.
       { apply SRCC. }
@@ -694,16 +583,16 @@ Section SimRelAddJF.
       cdes BSTEP_; cdes SAJF.
       erewrite ESstep.step_add_jf_jfe; eauto.
       rewrite dom_union. unionL. 
-      { eapply jfe_fI. apply SRCC. }
-      
+      { eapply jfe_ex_iss. apply SRCC. }
       erewrite sim_add_jf_jfe_delta_dom; eauto.
-      erewrite <- set_collect_eq_dom 
-        with (g := h).
-      2 : eapply eq_dom_mori; try eapply hfeq; eauto; red; basic_solver 10.
       etransitivity.
       2 : eapply ES.ew_eqvW; auto.
       { basic_solver. }
-      eapply fI_EW; apply SRCC.
+      apply set_subset_inter_r. split.
+      { erewrite Execution.ex_inE with (S := S) (X := X).
+        { basic_solver. }
+        apply SRCC. }
+      eapply ex_iss_inW. apply SRCC.
     Qed.
 
   End SimRelAddJFProps. 
